

**Theorem 1** (Monotonicity). *For all  $t \geq 0$ , the risk mass  $\theta$  is non-increasing:*

$$\theta_{t+1} \leq \theta_t.$$

*Proof.* **Step 1: Recursive Definition.**

The risk mass at time  $t + 1$  is defined by the Fading Operator  $F(\theta_t, d_t)$ :

$$\theta_{t+1} = \theta_{\min} + (\theta_t - \theta_{\min}) \exp(-\lambda_s d_t).$$

**Step 2: Exponential Bounds.**

Since  $\lambda_s > 0$  and  $d_t \geq 0$ , the exponential term satisfies:

$$0 \leq \exp(-\lambda_s d_t) \leq 1.$$

**Step 3: Inequality Substitution.**

By the Boundedness Axiom,  $(\theta_t - \theta_{\min}) \geq 0$ . Multiplying by the exponential term:

$$(\theta_t - \theta_{\min}) \exp(-\lambda_s d_t) \leq (\theta_t - \theta_{\min}).$$

**Step 4: Final Comparison.**

Adding  $\theta_{\min}$  to both sides:

$$\theta_{\min} + (\theta_t - \theta_{\min}) \exp(-\lambda_s d_t) \leq \theta_{\min} + (\theta_t - \theta_{\min}) = \theta_t.$$

Hence:

$$\theta_{t+1} \leq \theta_t.$$

□